v4.33.1-optimized/playground/Playground/LoxTests.lean
@@ -1,0 +1,8 @@
+import Playground.Lox
+
+
+theorem matchChar_prop (c : Char) (s : State) : (matchChar c).run s =
+  if s.input[s.current]? = some c then
+    (true, { s with current := s.current + 1 })
+  else
+    (false, s) := by sorry
